updated interp_commute_tmp1.v, added recursive case

proofs/itrees/interp_commute_tmp1.v
@@ -36,17 +36,10 @@ Section IEquiv0.
 
 (* simplest case: the two handlers are independent *)
 Context {E D1 D2: Type -> Type}. 
-Context (Hnd1 : forall T, D1 T -> itree E T)
-        (Hnd2 : forall T, D2 T -> itree E T).
+Context (Hnd1 : D1 ~> itree E) (Hnd2 : D2 ~> itree E).
 
 Definition join_hndl : (D1 +' D2) +' E ~> itree E :=
-  fun T d => match d with
-             | inl1 (inl1 d1) => Hnd1 d1
-             | inl1 (inr1 d2) => Hnd2 d2
-             | inr1 e => trigger e end.
-
-Definition interp_joinI : itree ((D1 +' D2) +' E) ~> itree E :=
-  fun T t => interp join_hndl t.  
+  case_ (case_ Hnd1 Hnd2) (id_ E).
 
 Definition interp_join : itree (D1 +' D2 +' E) ~> itree E :=
   fun T t => interp join_hndl (translate (@sum_lassoc D1 D2 E) t).  
@@ -97,17 +90,13 @@ Section IEquiv1.
 
 (* Hnd1 depends on D2 *)  
 Context {E D1 D2: Type -> Type}. 
-Context (Hnd1 : forall T, D1 T -> itree (D2 +' E) T)
-        (Hnd2 : forall T, D2 T -> itree E T).
+Context (Hnd1 : D1 ~> itree (D2 +' E)) (Hnd2 : D2 ~> itree E).
 
 Definition join_dhndl : (D1 +' D2) +' E ~> itree (D2 +' E) :=
   fun T d => match d with
              | inl1 (inl1 d1) => Hnd1 d1
              | inl1 (inr1 d2) => translate inr1 (Hnd2 d2)
              | inr1 e => trigger e end.
-
-Definition interp_djoinI : itree ((D1 +' D2) +' E) ~> itree (D2 +' E) :=
-  fun T t => interp join_dhndl t.  
 
 Definition interp_djoin : itree (D1 +' D2 +' E) ~> itree E :=
   fun T t => interp (ext_handler Hnd2)
@@ -132,7 +121,7 @@ Proof.
   }
   { setoid_rewrite interp_vis. 
     setoid_rewrite interp_bind.
-    unfold join_dhndl; simpl.
+     unfold join_dhndl; simpl.
     setoid_rewrite interp_tau.
     guclo eqit_clo_bind.
     econstructor 1 with (RU := eq); simpl.
@@ -160,28 +149,67 @@ Section IEquiv2.
 
 (* Hnd1 depends on D2 and it is recursive *)  
 Context {E D1 D2: Type -> Type}. 
-Context (Hnd1 : forall T, D1 T -> itree (D1 +' (D2 +' E)) T)
-        (Hnd2 : forall T, D2 T -> itree E T).
+Context (Hnd1 : D1 ~> itree (D1 +' (D2 +' E))) (Hnd2 : D2 ~> itree E).
 
-Definition join_rhndl : (D1 +' D2) ~> itree ((D1 +' D2) +' E) :=
+(* moves D2 event to non-recursive position, leave recursive D2 as
+   padding *)
+Definition pad3 : (D1 +' D2) +' E ~> (D1 +' D2) +' D2 +' E :=
+  fun T d => match d with
+             | inl1 (inl1 d1) => inl1 (inl1 d1)
+             | inl1 (inr1 d2) => inr1 (inl1 d2)                          
+             | inr1 e => inr1 (inr1 e) end.
+
+(* moves D2 events to non-recursive position, introduces recursive D2
+   as padding *)
+Definition pad3A : D1 +' D2 +' E ~> (D1 +' D2) +' D2 +' E :=
+  fun T d => match d with
+             | inl1 d1 => inl1 (inl1 d1)
+             | inr1 d2 => inr1 d2 end.
+
+Definition pad3C : D1 +' D2 +' E ~> (D1 +' D2) +' D2 +' E :=
+  fun T e => pad3 ((@sum_lassoc D1 D2 E) _ e).
+
+(* handle both D1 and D2 events *)
+Definition rjhnd : (D1 +' D2) ~> itree ((D1 +' D2) +' E) :=
   fun T d => match d with
              | inl1 d1 => translate (@sum_lassoc D1 D2 E) (Hnd1 d1)
              | inr1 d2 => translate inr1 (Hnd2 d2) end.
 
-Definition interp_rjoinI : itree ((D1 +' D2) +' E) ~> itree E :=
-  fun T t => interp_mrec join_rhndl t.  
+(* should be ok *)
+Definition rjhnd3B : (D1 +' D2) ~> itree ((D1 +' D2) +' (D2 +' E)) :=
+  fun T d => match d with
+             | inl1 d1 =>
+                 translate pad3C (Hnd1 d1)
+             | inr1 d2 => translate pad3 (trigger d2) end.
 
-Definition interp_rjoin : itree (D1 +' D2 +' E) ~> itree E :=
-  fun T t => interp_mrec join_rhndl (translate (@sum_lassoc D1 D2 E) t).
+(* delay joint handler *)
+Definition Hnd2X :  D2 +' E ~> itree E :=
+  fun _ e => Tau (match e with
+             | inl1 d2 => Hnd2 d2
+             | inr1 e0 => trigger e0 end).                  
 
-(* first try *)
-Lemma interp_rjoin_equiv {T} (t: itree (D1 +' D2 +' E) T) :
-  eutt eq (interp (ext_handler Hnd2) (interp_mrec Hnd1 t))
-          (interp_rjoin t).
+(* interprets D1 (recursive) events *)
+Definition interpR1 T (t: itree (D1 +' D2 +' E) T) : itree (D2 +' E) T :=
+   interp_mrec Hnd1 t.                      
+
+(* interprets both D1 and D2 events *)
+Definition interpR12 T (t: itree (D1 +' D2 +' E) T) : itree E T :=
+   interp_mrec rjhnd (translate (@sum_lassoc D1 D2 E) t).                      
+
+(* sure interprets only D1 events *)
+Definition interp3B T (t: itree (D1 +' D2 +' E) T) : itree (D2 +' E) T :=
+   interp_mrec rjhnd3B (translate pad3C t).                      
+  
+(* seems likely: neither can handle D2 events *)
+Lemma widen_aux1 T (t: itree (D1 +' D2 +' E) T) :
+  eutt eq (interpR1 t) (interp3B t).
+Admitted.
+
+(* as expected, the only snag is it requires Hnd2X (adding an extra
+   tau) rather than just (case_ Hnd2 (id_ E)) *)
+Lemma widen_aux2 T (t: itree (D1 +' D2 +' E) T) :
+  eutt eq (interp Hnd2X (interp3B t)) (interpR12 t). 
 Proof.
-  setoid_rewrite interp_mrec_as_interp.
-  setoid_rewrite interp_translate.
-  setoid_rewrite interp_interp.  
   revert t.
   ginit. gcofix CIH.
   intros t.
@@ -193,63 +221,271 @@ Proof.
   { gstep; red. simpl; econstructor; simpl.
     gfinal. left. eapply CIH.
   }
-  { setoid_rewrite interp_vis. 
-    guclo eqit_clo_bind.
-    econstructor 1 with (RU := eq).
-    { destruct e as [d1 | [d2 | e]]; simpl; try reflexivity.
-      { setoid_rewrite mrec_as_interp.
-        unfold join_rhndl at 2; simpl.
-        setoid_rewrite interp_interp.
-        setoid_rewrite interp_translate.
-        eapply eutt_interp; try reflexivity.
-        unfold eq2, Eq2_Handler, eutt_Handler.
-        intros T0 a.
-        (* PROBLEM: circular reasoning not covered by CIH *)
-        admit.
-      }
-      { setoid_rewrite interp_trigger.
-        setoid_rewrite mrec_as_interp.
-        admit.
-      }
-      { setoid_rewrite interp_trigger. reflexivity. }
-    }
-    { intros u1 u2 hh.
-      inv hh.
+  { unfold interpR12.
+    destruct e as [d1 | [d2 | e]]; simpl.
+    { unfold interp3B.         
+      rewrite unfold_translate; simpl.    
+      rewrite unfold_interp_mrec; simpl.
+      setoid_rewrite interp_tau.
+      unfold interpR12.
+      setoid_rewrite unfold_translate at 3; simpl.    
+      setoid_rewrite unfold_interp_mrec at 2; simpl.
+      setoid_rewrite <- translate_bind.
+      unfold interpR12, interp3B in CIH.
       gstep; red.
       econstructor.
+      gfinal. left.
+      eapply CIH.
+    }
+    { unfold interp3B, Hnd2X.
+      setoid_rewrite translate_vis; simpl.
+      setoid_rewrite unfold_interp_mrec. simpl.
+      setoid_rewrite interp_vis; simpl.
+      setoid_rewrite interp_tau.
+      setoid_rewrite interp_mrec_bind.
+      setoid_rewrite bind_tau.
+      gstep; red.
+      econstructor.
+      guclo eqit_clo_bind.
+      econstructor 1 with (RU := eq).
+      { setoid_rewrite interp_mrec_as_interp.
+        setoid_rewrite interp_translate; simpl.
+        setoid_rewrite interp_trigger_h.
+        reflexivity.
+      }
+      { intros u1 u2 hh.
+        inv hh.
+        repeat rewrite tau_euttge.
+        gfinal; left.
+        eapply CIH.
+       } 
+    }
+    { unfold interp3B, interpR12.
+      setoid_rewrite unfold_translate; simpl.
+      setoid_rewrite unfold_interp_mrec; simpl.
+      setoid_rewrite unfold_interp; simpl.
+      setoid_rewrite interp_tau; simpl.
+      unfold Hnd2X.
+      setoid_rewrite bind_tau.
+      rewrite tau_euttge.
+      setoid_rewrite bind_trigger.
+      gstep; red. constructor.
+      unfold id; intros v.
+      gstep; red.
+      econstructor.
+      guclo eqit_clo_trans.
+      econstructor.
+      { instantiate (2:=eq).
+        instantiate (1:= 
+           (interp Hnd2X 
+            (interp_mrec rjhnd3B (translate pad3C (k v))))).
+        setoid_rewrite tau_euttge.
+        reflexivity.
+      }
+      { instantiate (2:=eq).
+        reflexivity.
+      }
+      { gfinal. left.
+        eapply CIH.
+      }
+      { intros x x' y H. inv H; eauto. }
+      { intros x y y' H. inv H; eauto. }
+    }
+  }  
+Qed.    
+
+Lemma case_widen T (t : itree (D2 +' E) T) :
+  eutt eq (interp (case_ Hnd2 (id_ E)) t) (interp Hnd2X t).
+Proof.
+  revert t.
+  ginit. gcofix CIH.
+  intros t.
+  setoid_rewrite (itree_eta_ t).
+  remember (observe t) as ot.
+  destruct ot.
+  { setoid_rewrite interp_ret.
+    gstep; red; constructor; auto.
+  }
+  { setoid_rewrite interp_tau.
+    gstep; red; constructor.
+    gfinal; left. eapply CIH.
+  }
+  { setoid_rewrite interp_vis.
+    guclo eqit_clo_bind.
+    econstructor 1 with (RU := eq).
+    { unfold Hnd2X; simpl.
+      rewrite tau_euttge. reflexivity. }
+    { intros u1 u2 hh. inv hh.
+      gstep; red. constructor.
       gfinal; left.
       eapply CIH.
     }
-  }
-Abort.    
+  }  
+Qed.    
 
-(* second try *)
-Lemma interp_rjoin_equiv {T} (t: itree (D1 +' D2 +' E) T) :
-  eutt eq (interp (ext_handler Hnd2) (interp_mrec Hnd1 t))
-          (interp_rjoin t).
+(* our goal: *)
+Lemma widen_main T (t: itree (D1 +' D2 +' E) T) :
+  eutt eq (interp (case_ Hnd2 (id_ E)) (interpR1 t)) (interpR12 t). 
 Proof.
-  unfold interp_rjoin.  
-  set (HndE := (fun T d => translate (@inr1 D2 E) (@Hnd2 T d))).
+  rewrite widen_aux1.
+  rewrite <- widen_aux2.
+  revert t.
+  ginit. gcofix CIH.
+  intro t.
+  setoid_rewrite (itree_eta_ t).
+  remember (observe t) as ot.
+  destruct ot.
+  { unfold interp3B; simpl.
+    setoid_rewrite translate_ret.
+    setoid_rewrite unfold_interp_mrec; simpl.
+    setoid_rewrite interp_ret.
+    gstep; red.
+    econstructor; auto.
+  }
+  { unfold interp3B; simpl.
+    setoid_rewrite translate_tau.
+    setoid_rewrite unfold_interp_mrec; simpl.
+    setoid_rewrite interp_tau.
+    gstep; red.
+    econstructor.
+    gfinal. left.
+    eapply CIH.
+  }
+  { unfold interp3B; simpl.
+    setoid_rewrite translate_vis.
+    setoid_rewrite unfold_interp_mrec; simpl.
+    destruct e as [d1 | [d2 | e]]; simpl.
+    { setoid_rewrite interp_tau.
+      gstep; red.
+      econstructor.
+      setoid_rewrite interp_mrec_bind. 
+      setoid_rewrite interp_bind.
+      guclo eqit_clo_bind.
+      econstructor 1 with (RU := eq).
+      { generalize (interp_mrec rjhnd3B (translate pad3C (Hnd1 d1))).
+        intro t1.
+        eapply case_widen.
+      }
+      { intros u1 u2 hh. inv hh.
+        gfinal; left. eapply CIH.
+      }
+    }
+    { setoid_rewrite interp_vis.
+      guclo eqit_clo_bind.
+      econstructor 1 with (RU := eq).
+      { unfold Hnd2X; simpl.
+        rewrite tau_euttge. reflexivity. }
+      { intros u1 u2 hh. inv hh.
+        gstep; red.
+        econstructor.
+        setoid_rewrite interp_tau.
+        gstep; red.
+        econstructor.
+        gfinal; left. eapply CIH.
+      }
+    }  
+    { setoid_rewrite interp_vis.
+      guclo eqit_clo_bind.
+      econstructor 1 with (RU := eq).
+      { unfold Hnd2X; simpl.
+        rewrite tau_euttge. reflexivity. }
+      { intros u1 u2 hh. inv hh.
+        gstep; red.
+        econstructor.
+        setoid_rewrite interp_tau.
+        gstep; red.
+        econstructor.
+        gfinal; left. eapply CIH.
+      } 
+    }
+  }  
+Qed.    
 
-(* widen  to 
 
-   (interp (ext_handler Hnd2) (interp_rjoin (free2 t)))
+(**************************************************************)
 
-   (interp (ext_handler Hnd2) (free2 (interp_rjoin t)))
+(* USELESS STUFF *)
 
+(* introduce non-recursive D2 as padding *)
+Definition pad2 : (D1 +' D2) +' E ~> (D1 +' D2) +' D2 +' E :=
+  fun T d => match d with
+             | inl1 d12 => inl1 d12
+             | inr1 e => inr1 (inr1 e) end.
+
+(* does not handle D2 events but moves them to non-recursive position
 *)
-  
-(*  setoid_rewrite interp_mrec_as_interp at 2.
-  rewrite interp_translate. *)
-  
-  setoid_rewrite free_widening_lemma at 1.
+Definition rjhndX : (D1 +' D2) ~> itree ((D1 +' D2) +' (D2 +' E)) :=
+  fun T d => match d with
+             | inl1 d1 =>
+                 translate pad2 (translate (@sum_lassoc D1 D2 E) (Hnd1 d1))
+             | inr1 d2 => trigger (inl1 d2) end.
 
-  Fail instantiate (1 :=  (fun T d => translate inr1 (Hnd2 d))).
-  
- (* problem with the type of free_widening_lemma: to be fixed *)
-  Check @free_widening_lemma.
-Admitted.
+(* moves D2 events to recursive position, introduces non-recursive D2
+   as padding *)
+Definition pad2A : D1 +' D2 +' E ~> (D1 +' D2) +' D2 +' E :=
+  fun T d => match d with
+             | inl1 d1 => inl1 (inl1 d1)
+             | inr1 (inl1 d2) => inl1 (inr1 d2)
+             | inr1 (inr1 e) => inr1 (inr1 e) end.
 
+Definition pad2C : D1 +' D2 +' E ~> (D1 +' D2) +' D2 +' E :=
+  fun T e => pad2 ((@sum_lassoc D1 D2 E) _ e).
+
+Definition rjhnd2A : (D1 +' D2) ~> itree ((D1 +' D2) +' (D2 +' E)) :=
+  fun T d => match d with
+             | inl1 d1 =>
+                 translate pad2C (Hnd1 d1)
+             | inr1 d2 => trigger (inl1 d2) end.
+
+Lemma pad_check2 T (e: (D1 +' D2 +' E) T)  : pad3A e = pad3C e.
+  unfold pad3C.
+  destruct e as [d1 | [d2 | e]]; simpl; eauto.
+Qed.
+
+Lemma pad_check3 T (e: (D1 +' D2 +' E) T)  : pad2A e = pad2C e.
+  unfold pad2C.
+  destruct e as [d1 | [d2 | e]]; simpl; eauto.
+Qed.
+
+(* test *)
+Definition rjhnd2B : (D1 +' D2) ~> itree ((D1 +' D2) +' (D2 +' E)) :=
+  fun T d => match d with
+             | inl1 d1 =>
+                 translate pad2C (Hnd1 d1)
+             | inr1 d2 => translate pad2 (trigger d2) end.
+
+Definition rjhnd3A : (D1 +' D2) ~> itree ((D1 +' D2) +' (D2 +' E)) :=
+  fun T d => match d with
+             | inl1 d1 =>
+                 translate pad3C (Hnd1 d1)
+             | inr1 d2 => trigger (inl1 d2) end.
+
+Definition rjhnd3Br : (D1 +' D2) ~> itree ((D1 +' D2) +' (D2 +' E)) :=
+  fun T d => match d with
+             | inl1 d1 =>
+                 translate pad3C (Hnd1 d1)
+             | inr1 d2 => translate pad3 (trigger (inl1 (inr1 d2))) end.
+
+(* handle both D1 and D2 events *)
+Definition rjhndY : (D1 +' D2) ~> itree ((D1 +' D2) +' (D2 +' E)) :=
+  fun T d => match d with
+             | inl1 d1 =>
+                 translate pad2 (translate (@sum_lassoc D1 D2 E) (Hnd1 d1))
+             | inr1 d2 => translate inr1 (translate inr1 (Hnd2 d2)) end.
+
+(* inititally interprets only D1 events, as pad3A has moved D2 to
+   non-recursive position. However, interprets D2 events arising from
+   D1 *)
+Definition interpR1Y T (t: itree (D1 +' D2 +' E) T) : itree (D2 +' E) T :=
+   interp_mrec rjhndY (translate pad3A t).                      
+
+(* sure interprets only D1 events; should work also with pad2A *)
+Definition interpR1X0 T (t: itree (D1 +' D2 +' E) T) : itree (D2 +' E) T :=
+   interp_mrec rjhndX (translate pad3A t).                      
+
+(* sure interprets only D1 events; should work also with pad2A *)
+Definition interpR1X T (t: itree (D1 +' D2 +' E) T) : itree (D2 +' E) T :=
+   interp_mrec rjhndX (translate pad3C t).                      
 
 End IEquiv2.
 
